Continuing locals

theories/c_lang/lang.v
@@ -1,5 +1,5 @@
 From stdpp Require Export binders strings options.
-From stdpp Require Import gmap.
+From stdpp Require Import gmap finite.
 From iris.algebra Require Export ofe.
 From iris.heap_lang Require Export locations.
 From iris.prelude Require Import options.
@@ -38,6 +38,7 @@ Inductive expr :=
   | Let (x : binder) (e1 e2 : expr)
   (* Local variables *)
   | AdressOf (x : string)
+  | AllocFrame (f : gset string) (e : expr)
   (* Memory *)
   | Load (e : expr)
   | Store (e0 e1 : expr) (* e0 <- e1 *)
@@ -57,6 +58,7 @@ Definition expr_rect (P : expr → Type) :
   → (∀ x : string, P (Var x))
   → (∀ (x : binder) (e1 : expr), P e1 → ∀ e2 : expr, P e2 → P (Let x e1 e2))
   → (∀ x : string, P (AdressOf x))
+  → (∀ (f : gset string) (e : expr), P e → P (AllocFrame f e))
   → (∀ e : expr, P e → P (Load e))
   → (∀ e0 : expr, P e0 → ∀ e1 : expr, P e1 → P (Store e0 e1))
   → (∀ e1 : expr, P e1 → P (Malloc e1))
@@ -68,22 +70,23 @@ Definition expr_rect (P : expr → Type) :
   → (∀ e0 : expr, P e0 → ∀ ee : list expr, (forall ei, In2 ei ee -> P ei) -> P (FunCall e0 ee))
   → ∀ e : expr, P e.
 Proof.
-  refine (fun H1 H2 H3 H4 H5 H6 H7 H8 H9 H10 H11 H12 H13 => _).
+  refine (fun H1 H2 H3 H4 H5 H6 H7 H8 H9 H10 H11 H12 H13 H14 => _).
   refine (fix IH e {struct e} : P e := _).
   refine (match e as e0 return (P e0) with
      | Val v => H1 v
      | Var x => H2 x
      | Let x0 e3 e4 => H3 x0 e3 (IH e3) e4 (IH e4)
      | AdressOf x => H4 x
-     | Load e1 => H5 e1 (IH e1)
-     | Store e2 e3 => H6 e2 (IH e2) e3 (IH e3)
-     | Malloc e0 => H7 e0 (IH e0)
-     | Free e2 e3 => H8 e2 (IH e2) e3 (IH e3)
-     | UnOp op0 e1 => H9 op0 e1 (IH e1)
-     | BinOp op0 e3 e4 => H10 op0 e3 (IH e3) e4 (IH e4)
-     | If e3 e4 e5 =>  H11 e3 (IH e3) e4 (IH e4) e5 (IH e5)
-     | While e2 e3 => H12 e2 (IH e2) e3 (IH e3)
-     | FunCall e1 ee0 => H13 e1 (IH e1) ee0
+     | AllocFrame f e => H5 f e (IH e)
+     | Load e1 => H6 e1 (IH e1)
+     | Store e2 e3 => H7 e2 (IH e2) e3 (IH e3)
+     | Malloc e0 => H8 e0 (IH e0)
+     | Free e2 e3 => H9 e2 (IH e2) e3 (IH e3)
+     | UnOp op0 e1 => H10 op0 e1 (IH e1)
+     | BinOp op0 e3 e4 => H11 op0 e3 (IH e3) e4 (IH e4)
+     | If e3 e4 e5 =>  H12 e3 (IH e3) e4 (IH e4) e5 (IH e5)
+     | While e2 e3 => H13 e2 (IH e2) e3 (IH e3)
+     | FunCall e1 ee0 => H14 e1 (IH e1) ee0
           ((fix IHl (ll:list expr) {struct ll} : forall (x:expr) (i:In2 x ll), P x :=
             match ll as ll0 return forall (x:expr) (i:In2 x ll0), P x
             with nil => fun x i => False_rect _ i
@@ -98,6 +101,7 @@ Definition expr_ind (P : expr → Prop) :
   → (∀ x : string, P (Var x))
   → (∀ (x : binder) (e1 : expr), P e1 → ∀ e2 : expr, P e2 → P (Let x e1 e2))
   → (∀ (x : string), P (AdressOf x))
+  → (∀ (f : gset string) (e : expr), P e → P (AllocFrame f e))
   → (∀ e : expr, P e → P (Load e))
   → (∀ e0 : expr, P e0 → ∀ e1 : expr, P e1 → P (Store e0 e1))
   → (∀ e1 : expr, P e1 → P (Malloc e1))
@@ -109,22 +113,23 @@ Definition expr_ind (P : expr → Prop) :
   → (∀ e0 : expr, P e0 → ∀ ee : list expr, (forall ei, In ei ee -> P ei) -> P (FunCall e0 ee))
   → ∀ e : expr, P e.
 Proof.
-  refine (fun H1 H2 H3 H4 H5 H6 H7 H8 H9 H10 H11 H12 H13 => _).
+  refine (fun H1 H2 H3 H4 H5 H6 H7 H8 H9 H10 H11 H12 H13 H14 => _).
   refine (fix IH e {struct e} : P e := _).
   refine (match e as e0 return (P e0) with
      | Val v => H1 v
      | Var x => H2 x
      | Let x0 e3 e4 => H3 x0 e3 (IH e3) e4 (IH e4)
      | AdressOf x => H4 x
-     | Load e1 => H5 e1 (IH e1)
-     | Store e2 e3 => H6 e2 (IH e2) e3 (IH e3)
-     | Malloc e0 => H7 e0 (IH e0)
-     | Free e2 e3 => H8 e2 (IH e2) e3 (IH e3)
-     | UnOp op0 e1 => H9 op0 e1 (IH e1)
-     | BinOp op0 e3 e4 => H10 op0 e3 (IH e3) e4 (IH e4)
-     | If e3 e4 e5 =>  H11 e3 (IH e3) e4 (IH e4) e5 (IH e5)
-     | While e2 e3 => H12 e2 (IH e2) e3 (IH e3)
-     | FunCall e1 ee0 => H13 e1 (IH e1) ee0
+     | AllocFrame f e => H5 f e (IH e)
+     | Load e1 => H6 e1 (IH e1)
+     | Store e2 e3 => H7 e2 (IH e2) e3 (IH e3)
+     | Malloc e0 => H8 e0 (IH e0)
+     | Free e2 e3 => H9 e2 (IH e2) e3 (IH e3)
+     | UnOp op0 e1 => H10 op0 e1 (IH e1)
+     | BinOp op0 e3 e4 => H11 op0 e3 (IH e3) e4 (IH e4)
+     | If e3 e4 e5 =>  H12 e3 (IH e3) e4 (IH e4) e5 (IH e5)
+     | While e2 e3 => H13 e2 (IH e2) e3 (IH e3)
+     | FunCall e1 ee0 => H14 e1 (IH e1) ee0
           ((fix IHl (ll:list expr) {struct ll} : forall (x:expr) (i:In x ll), P x :=
             match ll as ll0 return forall (x:expr) (i:In x ll0), P x
             with nil => fun x i => False_rect _ i
@@ -183,6 +188,7 @@ Definition expr_rec (P : expr → Set) :
   → (∀ x : string, P (Var x))
   → (∀ (x : binder) (e1 : expr), P e1 → ∀ e2 : expr, P e2 → P (Let x e1 e2))
   → (∀ (x : string), P (AdressOf x))
+  → (∀ (f : gset string) (e : expr), P e → P (AllocFrame f e))
   → (∀ e : expr, P e → P (Load e))
   → (∀ e0 : expr, P e0 → ∀ e1 : expr, P e1 → P (Store e0 e1))
   → (∀ e1 : expr, P e1 → P (Malloc e1))
@@ -253,6 +259,7 @@ Proof.
      | Let x e1 e2, Let x' e1' e2' =>
         cast_if_and3 (decide (x = x')) (decide (e1 = e1')) (decide (e2 = e2'))
      | AdressOf x, AdressOf x' => cast_if (decide (x = x'))
+     | AllocFrame f e, AllocFrame f' e' => cast_if_and (decide (e = e')) (decide (f = f'))
      | Load e, Load e' => cast_if (decide (e = e'))
      | Store e1 e2, Store e1' e2' => cast_if_and (decide (e1 = e1')) (decide (e2 = e2'))
      | Malloc e, Malloc e' => cast_if (decide (e = e'))
@@ -295,45 +302,47 @@ Proof.
 Qed.
 
 Global Instance expr_countable : Countable expr.
-Proof. (* string + binder + un_op + bin_op + val *)
+Proof. (* string + binder + un_op + bin_op + val + gset string *)
  set (enc :=
    fix go e :=
      match e with
-     | Val v => GenNode 0 [GenLeaf (inr (inr (inr (inr v))))]
+     | Val v => GenNode 0 [GenLeaf $ inr $ inr $ inr $ inr $ inl v]
      | Var x => GenLeaf (inl x)
      | Let x e1 e2 => GenNode 1 [GenLeaf (inr (inl x)); go e1; go e2]
      | AdressOf x => GenNode 2 [GenLeaf (inl x)]
-     | Load e => GenNode 3 [go e]
-     | Store e1 e2 => GenNode 4 [go e1; go e2]
-     | Malloc e => GenNode 5 [go e]
-     | Free e1 e2 => GenNode 6 [go e1; go e2]
-     | UnOp op e => GenNode 7 [GenLeaf (inr (inr (inl op))); go e]
-     | BinOp op e1 e2 => GenNode 8 [GenLeaf (inr (inr (inr (inl op)))); go e1; go e2]
-     | If e0 e1 e2 => GenNode 9 [go e0; go e1; go e2]
-     | While e1 e2 => GenNode 10 [go e1; go e2]
-     | FunCall ef ea => GenNode 11 (go ef :: map go ea)
+     | AllocFrame f e => GenNode 3 [go e; GenLeaf $ inr $ inr $ inr $ inr $ inr f]
+     | Load e => GenNode 4 [go e]
+     | Store e1 e2 => GenNode 5 [go e1; go e2]
+     | Malloc e => GenNode 6 [go e]
+     | Free e1 e2 => GenNode 7 [go e1; go e2]
+     | UnOp op e => GenNode 8 [GenLeaf (inr (inr (inl op))); go e]
+     | BinOp op e1 e2 => GenNode 9 [GenLeaf $ inr $ inr $ inr $ inl op; go e1; go e2]
+     | If e0 e1 e2 => GenNode 10 [go e0; go e1; go e2]
+     | While e1 e2 => GenNode 11 [go e1; go e2]
+     | FunCall ef ea => GenNode 12 (go ef :: map go ea)
      end).
  set (dec :=
    fix go e :=
      match e with
-     | GenNode 0 [GenLeaf (inr (inr (inr (inr v))))] => Val v
+     | GenNode 0 [GenLeaf (inr (inr (inr (inr (inl v)))))] => Val v
      | GenLeaf (inl x) => Var x
      | GenNode 1 [GenLeaf (inr (inl x)); e1; e2] => Let x (go e1) (go e2)
      | GenNode 2 [GenLeaf (inl x)] => AdressOf x
-     | GenNode 3 [e] => Load (go e)
-     | GenNode 4 [e1; e2] => Store (go e1) (go e2)
-     | GenNode 5 [e] => Malloc (go e)
-     | GenNode 6 [e1; e2] => Free (go e1) (go e2)
-     | GenNode 7 [GenLeaf (inr (inr (inl op))); e] => UnOp op (go e)
-     | GenNode 8 [GenLeaf (inr (inr (inr (inl op)))); e1; e2] => BinOp op (go e1) (go e2)
-     | GenNode 9 [e0; e1; e2] => If (go e0) (go e1) (go e2)
-     | GenNode 10 [e1; e2] => While (go e1) (go e2)
-     | GenNode 11 (ef :: ea) => FunCall (go ef) (map go ea)
+     | GenNode 3 [e; GenLeaf (inr (inr (inr (inr (inr f)))))] => AllocFrame f (go e)
+     | GenNode 4 [e] => Load (go e)
+     | GenNode 5 [e1; e2] => Store (go e1) (go e2)
+     | GenNode 6 [e] => Malloc (go e)
+     | GenNode 7 [e1; e2] => Free (go e1) (go e2)
+     | GenNode 8 [GenLeaf (inr (inr (inl op))); e] => UnOp op (go e)
+     | GenNode 9 [GenLeaf (inr (inr (inr (inl op)))); e1; e2] => BinOp op (go e1) (go e2)
+     | GenNode 10 [e0; e1; e2] => If (go e0) (go e1) (go e2)
+     | GenNode 11 [e1; e2] => While (go e1) (go e2)
+     | GenNode 12 (ef :: ea) => FunCall (go ef) (map go ea)
      | _ => Val $ LitV (LitInt 0) (* dummy *)
      end).
  refine (inj_countable' enc dec _).
  refine (fix go (e : expr) {struct e} := _ ).
- destruct e as [ | | | | | | | | | | | |ef ee]; simpl; f_equal.
+ destruct e as [ | | | | | | | | | | | | |ef ee]; simpl; f_equal.
  1-17: done.
  all: unfold map; by induction ee as [|ex er ->]; simpl; f_equal.
 Qed.
@@ -398,6 +407,7 @@ Fixpoint subst_all (gv : gmap string expr) (ga : gmap string expr) (e : expr) : 
       | None   => e
       | Some k => k
       end
+  | AllocFrame f e => AllocFrame f (subst_all gv ga e) (* TODO: Delete all from f in gv and ga ? *)
   | Val _ => e
   | Let (BNamed s) e1 e2 =>
       Let (BNamed s) (subst_all gv ga e1) $ subst_all (delete s gv) (delete s ga) e2
@@ -487,37 +497,41 @@ Definition asTruth (v:val) : bool := match v with
   | LitV (LitFunPtr p) => true
   | LitV (LitNull) => false end.
 
+(** Function calls, local variables *)
+
 (*
  * Fails if :
  * - two variables share the same name
  * - a variable is used before it's declaration
+ * - a frame allocation is already present
  *)
-Fixpoint heap_locals (env : gset string) (e : expr) : option (gset string) :=
+Fixpoint stack_allocated (env : gset string) (e : expr) : option (gset string) :=
   match e with
   | Val _ => Some ∅
   | Var x => if decide (x ∈ env) then Some ∅ else None
   | AdressOf x => if decide (x ∈ env) then Some {[ x ]} else None
+  | AllocFrame f x => None
   | Let (BNamed x) e1 e2 =>
       if decide (x ∈ env) then None else
-      hl1 ← heap_locals env e1;
-      hl2 ← heap_locals (env ∪ {[ x ]}) e2;
+      hl1 ← stack_allocated env e1;
+      hl2 ← stack_allocated (env ∪ {[ x ]}) e2;
       Some (hl1 ∪ hl2)
   | Let BAnon e1 e2 | Store e1 e2 | Free e1 e2 | BinOp _ e1 e2 | While e1 e2 =>
-      hl1 ← heap_locals env e1;
-      hl2 ← heap_locals env e2;
+      hl1 ← stack_allocated env e1;
+      hl2 ← stack_allocated env e2;
       Some (hl1 ∪ hl2)
-  | Load e | Malloc e | UnOp _ e => heap_locals env e
+  | Load e | Malloc e | UnOp _ e => stack_allocated env e
   | If e1 e2 e3   =>
-      hl1 ← heap_locals env e1;
-      hl2 ← heap_locals env e2;
-      hl3 ← heap_locals env e3;
+      hl1 ← stack_allocated env e1;
+      hl2 ← stack_allocated env e2;
+      hl3 ← stack_allocated env e3;
       Some (hl1 ∪ hl2 ∪ hl3)
   | FunCall ef ea =>
       List.fold_left (fun acc e =>
-        hle  ← heap_locals env e;
+        hle  ← stack_allocated env e;
         acc' ← acc;
         Some (acc' ∪ hle))
-      ea (heap_locals env ef)
+      ea (stack_allocated env ef)
   end.
 
 (* Note that this way, a function where all arguments have the same name (say x), that returns x, returns the first argument *)
@@ -533,12 +547,30 @@ Definition apply_function (f : function) (av : list val) :=
   match f with
   | Fun an e =>
     match zip_args an av with
-    | Some σ =>
-        let locals := heap_locals (dom σ) e in
-        Some (subst_all σ ∅ e)
-    | _      => None
+    | Some args =>
+        match stack_allocated (dom args) e with
+        | Some frame =>
+            let args := filter (λ '(x, _), x ∉ frame) args in
+            Some (AllocFrame frame (subst_all args ∅ e))
+        | None => None
+        end
+    | _ => None
     end
   end.
+
+Fixpoint local_location (f : list string) (l : loc) : gmap string expr :=
+  match f with
+  | nil     => ∅
+  | v :: f' => {[v:=Val $ LitV $ LitLoc l]} ∪ (local_location f' (l +ₗ 1))
+  end.
+
+Definition allocate_frame (f : gset string) (e : expr) (l : loc) :=
+  let ll := Val $ LitV $ LitLoc l in
+  let ga := local_location (elements f) l in
+  let gv := fmap Load ga in
+  Let "res" (subst_all ∅ ga e)
+  $ Let BAnon (Free ll (Val $ LitV $ LitInt $ size f))
+  $ Var "res".
 
 Inductive head_step (p : gmap string function) : expr → c_state → expr → c_state → Prop :=
   | LetS x v1 e2 ee σ :
@@ -552,10 +584,13 @@ Inductive head_step (p : gmap string function) : expr → c_state → expr → c
      head_step p (Store (Val $ LitV $ LitLoc l) (Val w)) σ
                (Val $ LitV LitUnit) (state_upd_heap <[l:=Storing w]> σ)
   | MallocS n σ l :
-     (0 < n)%Z →
+     (0 ≤ n)%Z →
      (∀ i, (0 ≤ i)%Z → (i < n)%Z → σ !! (l +ₗ i) = None) →
      head_step p (Malloc (Val $ LitV $ LitInt n)) σ
                (Val $ LitV $ LitLoc l) (state_init_heap l n Uninitialized σ)
+  | AllocFrameS f e σ l :
+     (∀ i, (0 ≤ i)%Z → (i < size f)%Z → σ !! (l +ₗ i) = None) →
+     head_step p (AllocFrame f e) σ (allocate_frame f e l) (state_init_heap l (size f) Uninitialized σ)
   | FreeS l n σ :
      (∀ i, (0 ≤ i)%Z → (i < n)%Z → ∃ v, σ !! (l +ₗ i) = Some $ Some v) →
      head_step p (Free (Val $ LitV $ LitLoc l) (Val $ LitV $ LitInt n)) σ
@@ -599,7 +634,7 @@ Local Definition is_call e fn vs K :=
 
 Lemma alloc_fresh p n σ :
   let l := fresh_locs (dom σ) in
-  (0 < n)%Z →
+  (0 ≤ n)%Z →
   head_step p (Malloc ((Val $ LitV $ LitInt $ n))) σ
             (Val $ LitV $ LitLoc l) (state_init_heap l n Uninitialized σ).
 Proof.
@@ -888,7 +923,7 @@ Lemma unmap_val_map le lv : unmap_val le = Some lv → map Val lv = le.
 Proof.
   induction le in lv|-*.
   - intros H. injection H. intros <-. easy.
-  - cbn. destruct a. 2-13:congruence.
+  - cbn. destruct a. 2-14:congruence.
     destruct (unmap_val le) eqn:Heq. 2:congruence.
     intros H. injection H. intros <-. cbn. f_equal. now apply IHle.
 Qed.
